Prediction_error_free.v
@@ -10,32 +10,34 @@ Import ListNotations.
    FOR THE TWO TYPES OF PREDICTION ERRORS *)
 
 (* SP INVALID STATE CASE *)
-
-Definition all_sp_stacks_wf (g : grammar) (sps : list subparser) : Prop :=
-  forall sp, In sp sps -> lstack_wf g sp.(stack).
-
+(*
 Definition sp_ready_for_move (sp : subparser) : Prop :=
   match sp with
   | Sp _ _ (loc, locs) =>
-    (loc.(rsuf) = [] /\ locs = [])
-    \/ exists a suf, loc.(rsuf) = T a :: suf
+    (loc = SF [] /\ locs = [])
+    \/ exists a suf, loc = SF (T a :: suf)
   end.
 
 Definition all_sps_ready_for_move (sps : list subparser) : Prop :=
   forall sp, In sp sps -> sp_ready_for_move sp.
+ *)
 
 (* This definition can probably be merged with sp_ready_for_move *)
-Inductive stable_config : location_stack -> Prop :=
+Inductive stable_config : suffix_stack -> Prop :=
 | SC_empty :
-    forall pre,
-    stable_config (Loc pre [], [])
+    stable_config (SF [], [])
 | SC_terminal :
-    forall pre a suf frs,
-      stable_config (Loc pre (T a :: suf), frs).
+    forall a suf frs,
+      stable_config (SF (T a :: suf), frs).
+
+Hint Constructors stable_config.
+
+Definition all_stacks_stable sps :=
+  forall sp, In sp sps -> stable_config sp.(stack).
 
 Lemma spClosureStep_never_returns_SpInvalidState :
   forall g sp,
-    lstack_wf g sp.(stack)
+    suffix_stack_wf g sp.(stack)
     -> spClosureStep g sp <> SpClosureStepError SpInvalidState.
 Proof.
   intros g sp hw; unfold not; intros hs.
@@ -49,7 +51,7 @@ Lemma spClosure_never_returns_SpInvalidState :
          (sp   : subparser)
          (a'   : Acc lex_nat_pair (meas g sp)),
     pair = meas g sp
-    -> lstack_wf g sp.(stack)
+    -> suffix_stack_wf g sp.(stack)
     -> spClosure g sp a' <> inl SpInvalidState.
 Proof.
   intros g pair a'.
@@ -63,12 +65,12 @@ Proof.
     destruct heq' as [sp' [hi [hi' heq]]].
     eapply IH with (sp := sp'); eauto.
     + eapply spClosureStep_meas_lt; eauto.
-    + eapply spClosureStep_preserves_lstack_wf_invar; eauto.
+    + eapply spClosureStep_preserves_suffix_stack_wf_invar; eauto.
 Qed.
     
 Lemma closure_never_returns_SpInvalidState :
   forall g sps,
-    all_sp_stacks_wf g sps
+    all_suffix_stacks_wf g sps
     -> closure g sps <> inl SpInvalidState.
 Proof.
   intros g sps hw; unfold not; intros hc.
@@ -80,12 +82,12 @@ Proof.
 Qed.
 
 Lemma startState_never_returns_SpInvalidState :
-  forall g loc locs x suf,
-    lstack_wf g (loc, locs)
-    -> loc.(rsuf) = NT x :: suf
-    -> startState g x (loc, locs) <> inl SpInvalidState.
+  forall g fr frs x suf,
+    suffix_stack_wf g (fr, frs)
+    -> fr = SF (NT x :: suf)
+    -> startState g x (fr, frs) <> inl SpInvalidState.
 Proof.
-  intros g loc locs x suf hw heq; unfold not; intros hss.
+  intros g fr frs x suf hw heq; unfold not; intros hss.
   eapply closure_never_returns_SpInvalidState; eauto.
   intros sp hi.
   unfold initSps in hi.
@@ -94,9 +96,9 @@ Proof.
   (* LEMMA *)
   clear hss.
   inv hw; sis; subst.
-  - constructor; auto.
-    apply rhssForNt_in_iff; auto.
-  - constructor; auto.
+  - wf_upper_nil. 
+    apply rhssForNt_in_iff; eauto.
+  - wf_upper_nil. 
     apply rhssForNt_in_iff; auto.
 Qed.
 
@@ -110,20 +112,17 @@ Qed.
 
 Lemma moveSp_never_returns_SpInvalidState_for_ready_sp :
   forall g t sp,
-    sp_ready_for_move sp
+    stable_config sp.(stack)
     -> moveSp g t sp <> SpMoveError SpInvalidState.
 Proof.
   intros g t sp hr; unfold not; intros hm.
   unfold moveSp in hm.
-  dms; tc; sis.
-  - unfold sp_ready_for_move in hr; sis.
-    destruct hr as [[_ heq] | [a [suf heq]]]; inv heq.
-  - destruct hr as [[heq _] | [a [suf heq]]]; inv heq.
+  dms; tc; sis; inv hr.
 Qed.
 
 Lemma move_never_returns_SpInvalidState_for_ready_sps :
   forall g t sps,
-    all_sps_ready_for_move sps
+    all_stacks_stable sps
     -> move g t sps <> inl SpInvalidState.
 Proof.
   intros g t sps ha; unfold not; intros hm.
@@ -134,42 +133,41 @@ Proof.
   eapply moveSp_never_returns_SpInvalidState_for_ready_sp; eauto.
 Qed.
 
-Lemma moveSp_preserves_lstack_wf_invar :
+Lemma moveSp_preserves_suffix_stack_wf_invar :
   forall g t sp sp',
-    lstack_wf g sp.(stack)
+    suffix_stack_wf g sp.(stack)
     -> moveSp g t sp = SpMoveSucc sp'
-    -> lstack_wf g sp'.(stack).
+    -> suffix_stack_wf g sp'.(stack).
 Proof.
   intros g t sp sp' hw hm.
   unfold moveSp in hm; dms; tc; inv hm; sis.
-  inv hw; auto.
-  constructor; auto.
-  rewrite <- app_assoc; auto.
+  inv_suffix_frames_wf hw hi hw'; auto.
+  rewrite app_cons_group_l in hi; eauto.
 Qed.
 
-Lemma move_preserves_lstack_wf_invar :
+Lemma move_preserves_suffix_stack_wf_invar :
   forall g t sps sps',
-    all_sp_stacks_wf g sps
+    all_suffix_stacks_wf g sps
     -> move g t sps = inr sps'
-    -> all_sp_stacks_wf g sps'.
+    -> all_suffix_stacks_wf g sps'.
 Proof.
   intros g t sps sps' ha hm.
-  unfold all_sp_stacks_wf.
+  unfold all_suffix_stacks_wf.
   intros sp' hi.
   unfold move in hm.
   eapply aggrMoveResults_succ_in_input in hm; eauto.
   apply in_map_iff in hm.
   destruct hm as [sp [hm hi']].
-  eapply moveSp_preserves_lstack_wf_invar; eauto.
+  eapply moveSp_preserves_suffix_stack_wf_invar; eauto.
 Qed.
 
-Lemma spClosure_preserves_lstack_wf_invar :
+Lemma spClosure_preserves_suffix_stack_wf_invar :
   forall g pr (a : Acc lex_nat_pair pr) sp sp' a' sps',
     pr = meas g sp
-    -> lstack_wf g sp.(stack)
+    -> suffix_stack_wf g sp.(stack)
     -> spClosure g sp a' = inr sps'
     -> In sp' sps'
-    -> lstack_wf g sp'.(stack).
+    -> suffix_stack_wf g sp'.(stack).
 Proof.
   intros g pr a'.
   induction a' as [pr hlt IH]; intros sp sp' a sps' heq hw hs hi; subst.
@@ -182,49 +180,49 @@ Proof.
     destruct hi' as [sp'' [hi' [hi''' heq]]].
     eapply IH in heq; eauto.
     + eapply spClosureStep_meas_lt; eauto.
-    + eapply spClosureStep_preserves_lstack_wf_invar; eauto.
+    + eapply spClosureStep_preserves_suffix_stack_wf_invar; eauto.
 Qed.
   
-Lemma closure_preserves_lstack_wf_invar :
+Lemma closure_preserves_suffix_stack_wf_invar :
   forall g sps sps',
-    all_sp_stacks_wf g sps
+    all_suffix_stacks_wf g sps
     -> closure g sps = inr sps'
-    -> all_sp_stacks_wf g sps'.
+    -> all_suffix_stacks_wf g sps'.
 Proof.
   intros g sps sps' ha hc.
   unfold closure in hc.
-  unfold all_sp_stacks_wf.
+  unfold all_suffix_stacks_wf.
   intros sp' hi.
   eapply aggrClosureResults_succ_in_input in hc; eauto.
   destruct hc as [sps'' [hi' hi'']].
   apply in_map_iff in hi'.
   destruct hi' as [sp [hs hi']]; subst.
-  eapply spClosure_preserves_lstack_wf_invar; eauto.
+  eapply spClosure_preserves_suffix_stack_wf_invar; eauto.
   apply lex_nat_pair_wf.
 Qed.
 
-Lemma spClosureStepDone_ready_for_move :
+Lemma spClosureStepDone_stable_config :
   forall g sp,
     spClosureStep g sp = SpClosureStepDone
-    -> sp_ready_for_move sp.
+    -> stable_config sp.(stack).
 Proof.
   intros g sp hs.
   unfold spClosureStep in hs; dms; tc; sis; eauto.
 Qed.
 
-Lemma sp_in_spClosure_result_ready_for_move :
+Lemma sp_in_spClosure_result_stable_config :
   forall g pr (a : Acc lex_nat_pair pr) sp sp' a' sps',
     pr = meas g sp
     -> spClosure g sp a' = inr sps'
     -> In sp' sps'
-    -> sp_ready_for_move sp'.
+    -> stable_config sp'.(stack).
 Proof.
   intros g pr a'.
   induction a' as [pr hlt IH]; intros sp sp' a sps' heq hs hi; subst.
   apply spClosure_success_cases in hs.
   destruct hs as [[hd heq] | [sps'' [hs [crs [heq heq']]]]]; subst.
   - apply in_singleton_eq in hi; subst; auto.
-    eapply spClosureStepDone_ready_for_move; eauto.
+    eapply spClosureStepDone_stable_config; eauto.
   - eapply aggrClosureResults_succ_in_input in heq'; eauto.
     destruct heq' as [sps''' [hi' hi'']].
     eapply dmap_in in hi'; eauto.
@@ -233,27 +231,27 @@ Proof.
     eapply spClosureStep_meas_lt; eauto.
 Qed.
 
-Lemma sps_ready_for_move_after_closure :
+Lemma all_stacks_stable_after_closure :
   forall g sps sps',
     closure g sps = inr sps'
-    -> all_sps_ready_for_move sps'.
+    -> all_stacks_stable sps'.
 Proof.
   intros g sps sps' hc.
   unfold closure in hc.
-  unfold all_sps_ready_for_move.
+  unfold all_stacks_stable.
   intros sp' hi.
   eapply aggrClosureResults_succ_in_input in hc; eauto.
   destruct hc as [sps'' [hi' hi'']].
   apply in_map_iff in hi'.
   destruct hi' as [sp [hs hi']].
-  eapply sp_in_spClosure_result_ready_for_move; eauto.
+  eapply sp_in_spClosure_result_stable_config; eauto.
   apply lex_nat_pair_wf.
 Qed.
 
 Lemma llPredict'_never_returns_SpInvalidState :
   forall g ts sps,
-    all_sp_stacks_wf g sps
-    -> all_sps_ready_for_move sps
+    all_suffix_stacks_wf g sps
+    -> all_stacks_stable sps
     -> llPredict' g sps ts <> PredError SpInvalidState.
 Proof.
   intros g ts; induction ts as [| t ts IH]; intros sps ha ha'; unfold not; intros hl; sis.
@@ -266,31 +264,31 @@ Proof.
       eapply move_never_returns_SpInvalidState_for_ready_sps; eauto.
     + dmeq hc; tc.
       * inv hl.
-        eapply move_preserves_lstack_wf_invar in hm; eauto.
+        eapply move_preserves_suffix_stack_wf_invar in hm; eauto.
         eapply closure_never_returns_SpInvalidState; eauto.
       * eapply IH in hl; eauto.
-        -- eapply move_preserves_lstack_wf_invar in hm; eauto.
-           eapply closure_preserves_lstack_wf_invar; eauto.
-        -- eapply sps_ready_for_move_after_closure; eauto.
+        -- eapply move_preserves_suffix_stack_wf_invar in hm; eauto.
+           eapply closure_preserves_suffix_stack_wf_invar; eauto.
+        -- eapply all_stacks_stable_after_closure; eauto.
 Qed.
 
 Lemma stacks_wf_in_startState_result :
   forall g fr frs x suf sps,
-    lstack_wf g (fr, frs)
-    -> fr.(rsuf) = NT x :: suf
+    suffix_stack_wf g (fr, frs)
+    -> fr = SF (NT x :: suf)
     -> startState g x (fr, frs) = inr sps
-    -> all_sp_stacks_wf g sps.
+    -> all_suffix_stacks_wf g sps.
 Proof.
-  intros g [pre suf'] frs x suf sps hw heq hs; sis; subst.
-  eapply closure_preserves_lstack_wf_invar; eauto.
-  unfold all_sp_stacks_wf; intros sp hi.
-  eapply initSps_preserves_lstack_wf_invar; eauto.
+  intros g [suf'] frs x suf sps hw heq hs; sis; subst.
+  eapply closure_preserves_suffix_stack_wf_invar; eauto.
+  unfold all_suffix_stacks_wf; intros sp hi.
+  eapply initSps_preserves_suffix_stack_wf_invar; eauto.
 Qed.
 
 Lemma llPredict_never_returns_SpInvalidState :
   forall g fr frs x suf ts,
-    lstack_wf g (fr, frs)
-    -> fr.(rsuf) = NT x :: suf
+    suffix_stack_wf g (fr, frs)
+    -> fr = SF (NT x :: suf)
     -> llPredict g x (fr, frs) ts <> PredError SpInvalidState.
 Proof.
   intros g fr frs x suf ts hw heq; unfold not; intros hl.
@@ -301,7 +299,7 @@ Proof.
   - eapply llPredict'_never_returns_SpInvalidState; eauto.
     + eapply stacks_wf_in_startState_result; eauto.
     + unfold startState in hss.
-      eapply sps_ready_for_move_after_closure; eauto.
+      eapply all_stacks_stable_after_closure; eauto.
 Qed.
 
 (* LEFT RECURSION CASE *)
@@ -312,7 +310,7 @@ Lemma spClosureStep_LeftRecursion_facts :
     -> ~ NtSet.In x av
        /\ NtSet.In x (allNts g)
        /\ exists suf,
-           fr.(rsuf) = NT x :: suf.
+           fr = SF (NT x :: suf).
 Proof.
   intros g av pred fr frs x hs.
   unfold spClosureStep in hs; repeat dmeq h; tc; inv hs; sis.
@@ -322,9 +320,20 @@ Proof.
   - apply NtSet.mem_spec; auto.
 Qed.
 
+(* to do : clean up the next few lemmas *)
+
+Lemma nullable_path_two_head_frames :
+  forall g x y pre' suf',
+    In (x, pre' ++ NT y :: suf') g
+    -> nullable_gamma g pre'
+    -> nullable_path g (NT x) (NT y).
+Proof.
+  eauto.
+Qed.
+(*
 Lemma nullable_path_two_head_frames :
   forall g fr fr' frs y suf,
-    locations_wf g (fr :: fr' :: frs)
+    suffix_frames_wf g (fr :: fr' :: frs)
     -> nullable_gamma g fr.(rpre)
     -> fr.(rsuf) = NT y :: suf
     -> exists x suf',
@@ -334,76 +343,64 @@ Proof.
   intros g fr fr' frs y suf hw hn heq.
   inv hw; sis; subst; eauto.
 Qed.
-
+ *)
+(*
 Lemma stack_configuration_repr_nullable_path :
   forall g frs fr fr_cr x y suf suf',
-    locations_wf g (fr :: frs ++ [fr_cr])
-    -> nullable_gamma g fr.(rpre)
-    -> fr.(rsuf) = NT y :: suf
-    -> processed_symbols_all_nullable g frs
-    -> fr_cr.(rsuf) = NT x :: suf'
+    suffix_frames_nullable_path g (fr :: frs ++ [fr_cr])
+    -> fr = SF (NT y :: suf)
+    -> fr_cr = SF (NT x :: suf')
     -> nullable_path g (NT x) (NT y).
 Proof.
   intros g frs.
-  induction frs as [| fr' frs IH]; intros fr fr_cr x y suf suf' hw hn heq hp heq'.
-  - inv hw; sis.
-    inv heq'.
+  induction frs as [| fr' frs IH]; intros fr fr_cr x y suf suf' hn heq heq'; subst.
+  - inv hn; sis.
     eapply DirectPath; eauto.
-  - rename y into z.
-    pose proof hw as hw'.
-    eapply nullable_path_two_head_frames in hw'; eauto.
-    destruct hw' as [y [suf'' [heq'' hnp]]].
-    apply nullable_path_trans with (y := (NT y)); auto.
-    apply locations_wf_tl in hw.
-    inv hp; eapply IH in hw; eauto.
+  - inv hn; eapply nullable_path_trans; eauto.
 Qed.
-
-Lemma invars_imply_head_nt_available :
-  forall g av pred fr frs pre suf x,
-    fr = Loc pre (NT x :: suf)
+*)
+(*Lemma invars_imply_head_nt_available :
+  forall g av pred fr frs suf x,
+    fr = SF (NT x :: suf)
     -> no_left_recursion g
-    -> lstack_wf g (fr, frs)
+(*    -> suffix_frames_wf g (fr :: frs) *)
     -> unavailable_nts_invar g (Sp av pred (fr, frs))
     -> NtSet.In x (allNts g)
     -> NtSet.In x av.
 Proof.
-  intros g av pred fr frs pre suf x ? hn hw hu hi; subst.
+  intros g av pred fr frs suf x ? hn hu hi; subst.
   destruct (In_dec x av) as [hi' | hn']; auto.
   exfalso.
   apply hu in hn'; auto.
-  destruct hn' as [hng [frs_pre [fr_cr [frs_suf [suf' [heq [hp heq']]]]]]]; subst.
-  simpl in hw; rewrite app_group_endpoints_l in hw.
-  apply locations_wf_app_l in hw.
-  eapply stack_configuration_repr_nullable_path with (y := x) in hw; sis; eauto.
+  destruct hn' as [frs_pre [fr_cr [frs_suf [suf' [heq [hp heq']]]]]]; subst.
+  eapply stack_configuration_repr_nullable_path in hp; eauto.
   eapply hn; eauto.
-Qed.    
-
+Qed.
+ *)
 Lemma spClosureStep_never_finds_left_recursion :
   forall g sp x,
     no_left_recursion g
-    -> lstack_wf g sp.(stack)
     -> unavailable_nts_invar g sp
     -> spClosureStep g sp <> SpClosureStepError (SpLeftRecursion x).
 Proof.
-  intros g sp x hn hw hu; unfold not; intros hs.
-  destruct sp as [av pred (fr, frs)]; simpl in hw.
+  intros g [av pred (fr, frs)] x hn hu; unfold not; intros hs.
   pose proof hs as hs'.
   apply spClosureStep_LeftRecursion_facts in hs'.
-  destruct hs' as [hn' [hi [suf heq]]]; subst.
-  unfold spClosureStep in hs; dms; tc; sis; subst.
-  inv heq.
-  eapply invars_imply_head_nt_available with (pred := pred) in hi; eauto.
+  destruct hs' as [hn' [hi [suf' heq]]]; subst.
+  apply hu in hn'; auto.
+  destruct hn' as (frs_pre & fr_cr & frs_suf & suf & ? & ? & hf); subst.
+  eapply frames_repr_grammar_nullable_path in hf; eauto.
+  firstorder.
 Qed.
-  
+
 Lemma spClosure_never_finds_left_recursion :
   forall g pr (a : Acc lex_nat_pair pr) sp a' x,
     no_left_recursion g
-    -> lstack_wf g sp.(stack)
     -> unavailable_nts_invar g sp
     -> pr = meas g sp
     -> spClosure g sp a' <> inl (SpLeftRecursion x).
 Proof.
-  intros g pr a'; induction a' as [pr hlt IH]; intros sp a x hn hw hu heq; unfold not; intros hs; subst.
+  intros g pr a'; induction a' as [pr hlt IH]; intros sp a x hn hu heq; unfold not; intros hs; subst.
   apply spClosure_error_cases in hs.
   destruct hs as [hs | [sps [hs [crs [hc ha]]]]]; subst.
   - eapply spClosureStep_never_finds_left_recursion; eauto.
@@ -412,18 +409,16 @@ Proof.
     destruct ha as [sp' [hi [hi' hs']]].
     eapply IH with (sp := sp'); eauto.
     + eapply spClosureStep_meas_lt; eauto.
-    + eapply spClosureStep_preserves_lstack_wf_invar; eauto.
     + eapply spClosureStep_preserves_unavailable_nts_invar; eauto.
 Qed.
 
 Lemma closure_never_finds_left_recursion :
   forall g x sps,
     no_left_recursion g
-    -> all_sp_stacks_wf g sps
     -> sps_unavailable_nts_invar g sps
     -> closure g sps <> inl (SpLeftRecursion x).
 Proof.
-  intros g x sps hn hw hu; unfold not; intros hc.
+  intros g x sps hn hu; unfold not; intros hc.
   unfold closure in hc.
   apply aggrClosureResults_error_in_input in hc.
   apply in_map_iff in hc.
@@ -435,16 +430,13 @@ Qed.
 Lemma startState_never_finds_left_recursion :
   forall g x x' fr frs suf,
     no_left_recursion g
-    -> lstack_wf g (fr, frs)
-    -> fr.(rsuf) = NT x :: suf
+    -> fr = SF (NT x :: suf)
     -> startState g x (fr, frs) <> inl (SpLeftRecursion x').
 Proof.
-  intros g x x' [pre suf'] frs suf hn hw heq; unfold not; intros hs; sis; subst.
+  intros g x x' [suf'] frs suf hn heq; unfold not; intros hs; sis; inv heq; subst.
   eapply closure_never_finds_left_recursion; eauto.
-  - unfold all_sp_stacks_wf; intros sp hi.
-    eapply initSps_preserves_lstack_wf_invar; eauto.
-  - unfold sps_unavailable_nts_invar; intros sp hi.
-    eapply initSps_sat_unavailable_nts_invar; eauto.
+  unfold sps_unavailable_nts_invar; intros sp hi.
+  eapply initSps_sat_unavailable_nts_invar; eauto.
 Qed.
 
 Lemma moveSp_never_returns_SpLeftRecursion :
@@ -492,14 +484,13 @@ Proof.
   destruct hm as [sp [hm hi']].
   eapply unavailable_nts_invar_holds_after_moveSp; eauto.
 Qed.
-  
+
 Lemma llPredict'_never_returns_SpLeftRecursion :
   forall g ts sps x,
     no_left_recursion g
-    -> all_sp_stacks_wf g sps
     -> llPredict' g sps ts <> PredError (SpLeftRecursion x).
 Proof.
-  intros g ts; induction ts as [| t ts IH]; intros sps x hn hw; unfold not; intros hl; sis.
+  intros g ts; induction ts as [| t ts IH]; intros sps x hn; unfold not; intros hl; sis.
   - dm; tc; dm; tc.
     eapply handleFinalSubparsers_never_returns_error; eauto.
   - destruct sps as [| sp sps']; tc; dm; tc; dmeq hm; tc.
@@ -507,27 +498,20 @@ Proof.
       eapply move_never_returns_SpLeftRecursion; eauto.
     + dmeq hc.
       * inv hl.
-        pose proof hm as hm'.
-        eapply move_preserves_lstack_wf_invar in hm; eauto.
-        eapply unavailable_nts_invar_holds_after_move in hm'.
+        eapply unavailable_nts_invar_holds_after_move in hm.
         eapply closure_never_finds_left_recursion in hc; eauto.
       * eapply IH in hl; eauto.
-        eapply move_preserves_lstack_wf_invar in hm; eauto.
-        eapply closure_preserves_lstack_wf_invar; eauto.
 Qed.
-         
+
 Lemma llPredict_never_returns_SpLeftRecursion :
   forall g x x' fr frs ts suf,
     no_left_recursion g
-    -> lstack_wf g (fr, frs)
-    -> fr.(rsuf) = NT x :: suf
+    -> fr = SF (NT x :: suf)
     -> llPredict g x (fr, frs) ts <> PredError (SpLeftRecursion x').
 Proof.
-  intros g x x' fr frs ts suf hn hw heq; unfold not; intros hl.
+  intros g x x' fr frs ts suf hn heq; unfold not; intros hl.
   unfold llPredict in hl.
   dmeq hss.
-  - inv hl.
-    eapply startState_never_finds_left_recursion; eauto.
+  - inv hl; eapply startState_never_finds_left_recursion; eauto.
   - eapply llPredict'_never_returns_SpLeftRecursion; eauto.
-    eapply stacks_wf_in_startState_result; eauto.
 Qed.
